Final rework for PreStar

Lemke/FiniteAutomaton.thy
@@ -1,5 +1,9 @@
 section\<open>Finite Automata\<close>
 
+theory FiniteAutomaton
+  imports Main
+begin \<comment>\<open>begin-theory FiniteAutomaton\<close>
+
 text\<open>
   The fact that for a regular language \<open>L\<close>, the predecessors with respect to a context-free grammar
   \<open>pre\<^sup>*(L)\<close> is also regular has been discovered independently by many authors \cite{book1993string, buchi3105regular, caucal1992regular}.
@@ -8,10 +12,6 @@ text\<open>
   To reason about regular languages, a simple model of a non-deterministic finite automaton (NFA)
   without \<open>\<epsilon>\<close>-transitions is defined.
 \<close>
-
-theory FiniteAutomaton
-  imports Main
-begin \<comment>\<open>begin-theory FiniteAutomaton\<close>
 
 subsection\<open>Definition\<close>
 
@@ -42,7 +42,7 @@ lemma [code_unfold]:
   by fastforce
 
 text\<open>
-  A step from a single state \<open>q\<close> over a single symbol \<open>c\<close> is the set of all \<open>q'\<close>, where \<open>(q, c, q') \<in> \<delta>\<close>:
+  A step from a state \<open>q\<close> over a single symbol \<open>c\<close> is the set of all \<open>q'\<close>, such that \<open>(q, c, q') \<in> \<delta>\<close>:
 \<close>
 
 definition step :: "('s \<times> 't \<times> 's) set \<Rightarrow> 't \<Rightarrow> 's \<Rightarrow> 's set" where
@@ -53,7 +53,7 @@ text\<open>
 \<close>
 
 definition Step :: "('s \<times> 't \<times> 's) set \<Rightarrow> 't \<Rightarrow> 's set \<Rightarrow> 's set" where
-  "Step T c S = \<Union>((\<lambda>s. step T c s) ` S)"
+  "Step T c S = \<Union>(step T c ` S)"
 
 text\<open>
   Repeated steps of a word \<open>w\<close> consisting of multiple letters is achieved using a standard @{term fold}:
@@ -63,16 +63,20 @@ definition Steps :: "('s \<times> 't \<times> 's) set \<Rightarrow> 't list \<Ri
   "Steps T w s = fold (Step T) w s"
 
 text\<open>
-  However, we often only regard a single-starting state, for which the following abbreviation is introduced:
+  Often, merely a single starting-state is of relevance:
 \<close>
 
 abbreviation steps :: "('s \<times> 't \<times> 's) set \<Rightarrow> 't list \<Rightarrow> 's \<Rightarrow> 's set" where
   "steps T w s \<equiv> Steps T w {s}"
 
+text\<open>
+  We now prove some key properties of this step relation:
+\<close>
+
 lemma Step_union: "Step T w (S\<^sub>1 \<union> S\<^sub>2) = Step T w S\<^sub>1 \<union> Step T w S\<^sub>2"
   unfolding Step_def by blast
 
-lemma Steps_mono: "s\<^sub>1 \<subseteq> s\<^sub>2 \<Longrightarrow> Steps T w s\<^sub>1 \<subseteq> Steps T w s\<^sub>2"
+lemma Steps_subset: "s\<^sub>1 \<subseteq> s\<^sub>2 \<Longrightarrow> Steps T w s\<^sub>1 \<subseteq> Steps T w s\<^sub>2"
 proof (induction w arbitrary: s\<^sub>1 s\<^sub>2)
   case Nil thus ?case by (simp add: Steps_def)
 next
@@ -93,8 +97,8 @@ next
     by simp
 qed
 
-lemma [mono]: "mono (Steps T w)" (* TODO: give proper name to lemma *)
-  by (intro monoI, elim Steps_mono)
+lemma Steps_mono[mono]: "mono (Steps T w)"
+  by (intro monoI, elim Steps_subset)
 
 lemma Steps_path:
   assumes "q\<^sub>f \<in> Steps T w s"
@@ -112,7 +116,7 @@ next
 
   note \<open>q\<^sub>0 \<in> step T w q'\<close> and \<open>q\<^sub>f \<in> steps T ws q\<^sub>0\<close>
   then have "q\<^sub>f \<in> Steps T ws (step T w q')"
-    using Steps_mono[of "{q\<^sub>0}"] by blast
+    using Steps_subset[of "{q\<^sub>0}"] by blast
   moreover have "Steps T ws (step T w q') = steps T (w#ws) q'"
     by (simp add: Steps_def step_def Step_def)
   ultimately show ?case
@@ -145,7 +149,7 @@ proof -
   have "{q'} \<subseteq> Q'"
     using assms(1) by simp
   then have "Steps T w\<^sub>2 {q'} \<subseteq> Steps T w\<^sub>2 Q'"
-    using Steps_mono by blast
+    using Steps_subset by blast
   then have "q\<^sub>f \<in> Steps T w\<^sub>2 Q'"
     using assms(2) by fastforce
   moreover have "Q\<^sub>f = Steps T (w\<^sub>1@w\<^sub>2) Q\<^sub>0"
@@ -178,44 +182,65 @@ proof -
     by blast
 qed
 
+lemma Steps_noState: "Steps \<delta> w {} = {}"
+proof (induction w)
+  case Nil
+  then show ?case
+    by (simp add: Steps_def)
+next
+  case (Cons w ws)
+  moreover have "Steps \<delta> [w] {} = {}"
+    by (simp add: Steps_def Step_def)
+  ultimately show ?case
+    by (simp add: Steps_def)
+qed
+
 subsection\<open>Language\<close>
 
-abbreviation accepts :: "('s \<times> 't \<times> 's) set \<Rightarrow> 's \<Rightarrow> 's set \<Rightarrow> 't list \<Rightarrow> bool" where
-  "accepts T s F w \<equiv> (steps T w s \<inter> F \<noteq> {})"
+text\<open>
+  The language \<open>L(M)\<close> of a given automata \<open>M\<close> is defined as the set of words, that
+  reach at least one final state from a given starting state:
+\<close>
+
+abbreviation trans_accepts :: "('s \<times> 't \<times> 's) set \<Rightarrow> 's \<Rightarrow> 's set \<Rightarrow> 't list \<Rightarrow> bool" where
+  "trans_accepts T s F w \<equiv> (steps T w s \<inter> F \<noteq> {})"
+
+abbreviation nfa_accepts :: "('s, 't) nfa \<Rightarrow> 't list \<Rightarrow> bool" where
+  "nfa_accepts M \<equiv> trans_accepts (transitions M) (start M) (finals M)"
 
 lemma accepts_split3:
-  assumes "accepts T s F (w\<^sub>1@w\<^sub>2@w\<^sub>3)"
+  assumes "trans_accepts T s F (w\<^sub>1@w\<^sub>2@w\<^sub>3)"
   shows "\<exists>q' q'' q\<^sub>f. q' \<in> steps T w\<^sub>1 s \<and> q'' \<in> steps T w\<^sub>2 q' \<and> q\<^sub>f \<in> steps T w\<^sub>3 q'' \<and> q\<^sub>f \<in> F"
   using assms Steps_split3 by fast
 
-definition lang' :: "('s \<times> 't \<times> 's) set \<Rightarrow> 's \<Rightarrow> 's set \<Rightarrow> ('t list) set" where
-  "lang' T S F \<equiv> { w | w. accepts T S F w }"
+abbreviation trans_lang :: "('s \<times> 't \<times> 's) set \<Rightarrow> 's \<Rightarrow> 's set \<Rightarrow> ('t list) set" where
+  "trans_lang T S F \<equiv> { w. trans_accepts T S F w }"
 
-abbreviation lang :: "('s, 't) nfa \<Rightarrow> ('t list) set" where
-  "lang M \<equiv> lang' (transitions M) (start M) (finals M)"
+abbreviation nfa_lang :: "('s, 't) nfa \<Rightarrow> ('t list) set" where
+  "nfa_lang M \<equiv> trans_lang (transitions M) (start M) (finals M)"
 
 lemma nfa_lang_trans:
-  assumes "s' \<in> steps T w\<^sub>1 s" and "w\<^sub>2 \<in> lang' T s' F"
-  shows "(w\<^sub>1@w\<^sub>2) \<in> lang' T s F"
+  assumes "s' \<in> steps T w\<^sub>1 s" and "w\<^sub>2 \<in> trans_lang T s' F"
+  shows "(w\<^sub>1@w\<^sub>2) \<in> trans_lang T s F"
 proof -
   obtain q\<^sub>f where "q\<^sub>f \<in> steps T w\<^sub>2 s'" and "q\<^sub>f \<in> F"
-    using assms(2) unfolding lang'_def by blast
+    using assms(2) by blast
   moreover have "q\<^sub>f \<in> steps T (w\<^sub>1@w\<^sub>2) s"
     using assms(1) \<open>q\<^sub>f \<in> steps T w\<^sub>2 s'\<close> by (rule Steps_join)
   ultimately show ?thesis
-    unfolding lang'_def using \<open>q\<^sub>f \<in> F\<close> by blast
+    using \<open>q\<^sub>f \<in> F\<close> by blast
 qed
 
 lemma nfa_lang_split:
-  assumes "(w\<^sub>1@w\<^sub>2) \<in> lang' T q F"
-  obtains q' where "q' \<in> steps T w\<^sub>1 q" and "w\<^sub>2 \<in> lang' T q' F"
+  assumes "(w\<^sub>1@w\<^sub>2) \<in> trans_lang T q F"
+  obtains q' where "q' \<in> steps T w\<^sub>1 q" and "w\<^sub>2 \<in> trans_lang T q' F"
 proof -
   obtain q\<^sub>f where "q\<^sub>f \<in> steps T (w\<^sub>1@w\<^sub>2) q" and "q\<^sub>f \<in> F"
-    using assms unfolding lang'_def by blast
+    using assms by blast
   then obtain q' where "q' \<in> steps T w\<^sub>1 q" and "q\<^sub>f \<in> steps T w\<^sub>2 q'"
     using Steps_split by fast
-  moreover have "w\<^sub>2 \<in> lang' T q' F"
-    unfolding lang'_def using \<open>q\<^sub>f \<in> F\<close> calculation by blast
+  moreover have "w\<^sub>2 \<in> trans_lang T q' F"
+    using \<open>q\<^sub>f \<in> F\<close> calculation by blast
   ultimately show ?thesis
     using that by blast
 qed
@@ -230,7 +255,7 @@ next
   have "Step T\<^sub>1 w q\<^sub>1 \<subseteq> Step T\<^sub>2 w q\<^sub>2"
     unfolding Step_def step_def using assms(1) Cons(2) by blast
   then have "Steps T\<^sub>1 ws (Step T\<^sub>1 w q\<^sub>1) \<subseteq> Steps T\<^sub>1 ws (Step T\<^sub>2 w q\<^sub>2)"
-    by (rule Steps_mono)
+    by (rule Steps_subset)
   then have "Steps T\<^sub>1 ws (Step T\<^sub>1 w q\<^sub>1) \<subseteq> Steps T\<^sub>2 ws (Step T\<^sub>2 w q\<^sub>2)"
     using Cons(1) by blast
   then show ?case
@@ -257,14 +282,18 @@ proof -
     by (rule nfa_steps_mono)
 qed
 
-lemma nfa_lang_mono: "T\<^sub>1 \<subseteq> T\<^sub>2 \<Longrightarrow> lang' T\<^sub>1 s f \<subseteq> lang' T\<^sub>2 s f"
-  unfolding lang'_def using nfa_mono[of T\<^sub>1 T\<^sub>2] by fast
+lemma nfa_lang_mono: "T\<^sub>1 \<subseteq> T\<^sub>2 \<Longrightarrow> trans_lang T\<^sub>1 s f \<subseteq> trans_lang T\<^sub>2 s f"
+  using nfa_mono[of T\<^sub>1 T\<^sub>2] by fast
 
 subsection\<open>Reachable States\<close>
 
-type_synonym ('s, 't) Trans = "('s \<times> 't \<times> 's) set"
+text\<open>
+  The automata model is designed to work with datatypes with a potentially infinite universe.
+  Generating a finite set of reachable states (i.e., filter out the states that are of no interest)
+  is therefore a key factor to allow for automatic execution:
+\<close>
 
-definition reachable_from :: "('s, 't) Trans \<Rightarrow> 's \<Rightarrow> 's set" where
+definition reachable_from :: "('s \<times> 't \<times> 's) set \<Rightarrow> 's \<Rightarrow> 's set" where
   "reachable_from \<delta> q \<equiv> {q'. \<exists>w. q' \<in> steps \<delta> w q}"
 
 lemma reachable_from_computable: "reachable_from \<delta> q \<subseteq> {q} \<union> (snd ` snd ` \<delta>)"
@@ -352,6 +381,365 @@ next
   qed
   then show "q' \<in> reachable_from \<delta> q"
     by (simp add: reachable_from_def)
+qed
+
+subsection\<open>Merging Automata\<close>
+
+text\<open>
+  We will later provide concrete example of automata accepting specific languages.
+  While proving words that satisfy certain requirements are contained within a language
+  often is straight-forward, proving that the language only contains words satisfying
+  these requirements is a much more difficult task. The below lemma provides a powerful
+  tool to make these proofs manageable.
+\<close>
+
+text\<open>
+  Vividly speaking, this lemma shows that when two disjunct NFAs (or rather sets of transitions),
+  i.e. no states are shared, are connected via a single uni-directional bridge, every word that
+  reaches from the first set of states to the a state within the second state must, at some point,
+  pass this bridge, and have a prefix within the first set of states and a suffix within the
+  second set.
+\<close>
+
+text\<open>
+  This fact can later be used to prove behavior of inductively defined or merged automata.
+\<close>
+
+lemma nfa_merge:
+  assumes "s\<^sub>A \<in> A" and "f\<^sub>A \<in> A" and "s\<^sub>B \<in> B" and "f\<^sub>B \<in> B" and "A \<inter> B = {}"
+    and sideA: "\<forall>(q,c,q') \<in> \<delta>\<^sub>A. q \<in> A \<and> q' \<in> A"
+    and sideB: "\<forall>(q,c,q') \<in> \<delta>\<^sub>B. q \<in> B \<and> q' \<in> B"
+    and "f\<^sub>B \<in> steps (\<delta>\<^sub>A \<union> {(f\<^sub>A, c, s\<^sub>B)} \<union> \<delta>\<^sub>B) w s\<^sub>A"
+  shows "\<exists>w\<^sub>A w\<^sub>B. w = w\<^sub>A@[c]@w\<^sub>B \<and> f\<^sub>A \<in> steps \<delta>\<^sub>A w\<^sub>A s\<^sub>A \<and> f\<^sub>B \<in> steps \<delta>\<^sub>B w\<^sub>B s\<^sub>B"
+proof (insert assms; induction w arbitrary: s\<^sub>A)
+  case Nil
+  then have "steps (\<delta>\<^sub>A \<union> {(f\<^sub>A, c, s\<^sub>B)} \<union> \<delta>\<^sub>B) [] s\<^sub>A = {s\<^sub>A}"
+    by (simp add: Steps_def)
+  then show ?case
+    using Nil(8) Nil(1,4,5) by fast
+next
+  case (Cons a w)
+  define \<delta> where "\<delta> \<equiv> \<delta>\<^sub>A \<union> {(f\<^sub>A, c, s\<^sub>B)} \<union> \<delta>\<^sub>B"
+
+  \<comment> \<open>Obtain intermediate state after reading \<open>a\<close>:\<close>
+  note \<open>f\<^sub>B \<in> steps (\<delta>\<^sub>A \<union> {(f\<^sub>A, c, s\<^sub>B)} \<union> \<delta>\<^sub>B) (a#w) s\<^sub>A\<close>
+  then obtain q where a_step: "q \<in> steps \<delta> [a] s\<^sub>A"
+    and w_step: "f\<^sub>B \<in> steps \<delta> w q"
+    unfolding \<delta>_def using Steps_split by force
+
+  \<comment> \<open>There are now two options:\<close>
+  \<comment> \<open>1. \<open>a\<close> directly traverses the bridge to \<open>B\<close>, so \<open>a = c\<close>.\<close>
+  \<comment> \<open>2. \<open>a\<close> remains within \<open>A\<close> and we can use the IH.\<close>
+  then show ?case
+  proof (cases "(s\<^sub>A, a, q) \<notin> \<delta>\<^sub>A")
+    case True
+    moreover have "(s\<^sub>A, a, q) \<notin> \<delta>\<^sub>B"
+      using Cons(2,6,8) by fast
+    moreover have "(s\<^sub>A, a, q) \<in> \<delta>"
+      using a_step by (auto simp: Steps_def Step_def step_def)
+    ultimately have "s\<^sub>A = f\<^sub>A" and "a = c" and "q = s\<^sub>B"
+      unfolding \<delta>_def by simp+
+
+    have inB: "s\<^sub>B \<in> B \<Longrightarrow> f\<^sub>B \<in> steps \<delta> w s\<^sub>B \<Longrightarrow> f\<^sub>B \<in> steps \<delta>\<^sub>B w s\<^sub>B"
+    proof (induction w arbitrary: s\<^sub>B)
+      case Nil
+      then show ?case
+        by (simp add: Steps_def)
+    next
+      case (Cons x xs)
+      then obtain q where "f\<^sub>B \<in> steps \<delta> xs q" and "q \<in> steps \<delta> [x] s\<^sub>B"
+        using Steps_split by force
+      then have "(s\<^sub>B, x, q) \<in> \<delta>"
+        by (auto simp: Steps_def Step_def step_def)
+      moreover have "s\<^sub>B \<in> B"
+        using Cons by simp
+      ultimately have "(s\<^sub>B, x, q) \<in> \<delta>\<^sub>B" and "q \<in> B"
+        unfolding \<delta>_def using assms(2,5,6,7) by blast+
+      then have "q \<in> steps \<delta>\<^sub>B [x] s\<^sub>B"
+        by (auto simp: Steps_def Step_def step_def) force
+      moreover have "f\<^sub>B \<in> steps \<delta>\<^sub>B xs q"
+        using \<open>f\<^sub>B \<in> steps \<delta> xs q\<close> \<open>q \<in> B\<close> Cons by simp
+      ultimately show ?case
+        using Steps_join by force
+    qed
+
+    \<comment> \<open>The bridge is directly traversed, so \<open>A\<close> can be ignored:\<close>
+    have "a#w = []@[c]@w"
+      by (simp add: \<open>a = c\<close>)
+    moreover have "f\<^sub>A \<in> steps \<delta>\<^sub>A [] s\<^sub>A"
+      by (simp add: \<open>s\<^sub>A = f\<^sub>A\<close> Steps_def)
+    moreover have "f\<^sub>B \<in> steps \<delta>\<^sub>B w s\<^sub>B"
+      using w_step assms(3) inB by (simp add: \<open>q = s\<^sub>B\<close>)
+    ultimately show ?thesis
+      by blast
+  next
+    case False
+    then have a_step': "q \<in> steps \<delta>\<^sub>A [a] s\<^sub>A"
+      by (auto simp: Steps_def Step_def step_def, force)
+    then have "q \<in> A"
+      using False Cons(7) by fast
+
+    \<comment> \<open>Introduce the IH:\<close>
+    then have "\<exists>w\<^sub>A w\<^sub>B. w = w\<^sub>A @[c]@w\<^sub>B \<and> f\<^sub>A \<in> steps \<delta>\<^sub>A w\<^sub>A q \<and> f\<^sub>B \<in> steps \<delta>\<^sub>B w\<^sub>B s\<^sub>B"
+      by (rule Cons.IH; use Cons.prems w_step[unfolded \<delta>_def] in simp)
+    then obtain w\<^sub>A w\<^sub>B where "w = w\<^sub>A @[c]@w\<^sub>B" and "f\<^sub>A \<in> steps \<delta>\<^sub>A w\<^sub>A q" and "f\<^sub>B \<in> steps \<delta>\<^sub>B w\<^sub>B s\<^sub>B"
+      by blast
+    moreover have "f\<^sub>A \<in> steps \<delta>\<^sub>A (a#w\<^sub>A) s\<^sub>A"
+      using a_step' calculation(2) Steps_join by force
+    ultimately have "a#w = a#w\<^sub>A@[c]@w\<^sub>B \<and> f\<^sub>A \<in> steps \<delta>\<^sub>A (a#w\<^sub>A) s\<^sub>A \<and> f\<^sub>B \<in> steps \<delta>\<^sub>B w\<^sub>B s\<^sub>B"
+      by simp
+    then show ?thesis
+      by (intro exI) auto
+  qed
+qed
+
+subsection\<open>Concrete Automata\<close>
+
+text\<open>
+  We now present three concrete automata that accept certain languages.
+\<close>
+
+subsubsection\<open>Universe over specific Alphabet\<close>
+
+text\<open>
+  This automaton acceptes exactly the words that only contains
+  letters from a given alphabet.
+\<close>
+
+definition nfa_univ_trans :: "'s \<Rightarrow> 'a set \<Rightarrow> ('s \<times> 'a \<times> 's) set" where
+  "nfa_univ_trans q U \<equiv> {q} \<times> U \<times> {q}"
+
+lemma nfa_univ_trans_fin: "finite U \<Longrightarrow> finite (nfa_univ_trans q U)"
+  by (simp add: nfa_univ_trans_def)
+
+lemma nfa_univ_trans_correct1: "set w \<subseteq> U \<Longrightarrow> steps (nfa_univ_trans q U) w q = {q}"
+proof (induction w)
+  case Nil
+  then show ?case
+    by (simp add: Steps_def)
+next
+  case (Cons w ws)
+  then have "steps (nfa_univ_trans q U) [w] q = {q}"
+    unfolding nfa_univ_trans_def Steps_def Step_def step_def by fastforce
+  moreover have "steps (nfa_univ_trans q U) ws q = {q}"
+    using Cons by simp
+  ultimately show ?case
+    by (simp add: Steps_def)
+qed
+
+lemma nfa_univ_trans_correct2: "\<not> set w \<subseteq> U \<Longrightarrow> steps (nfa_univ_trans q U) w q = {}"
+proof (induction w)
+  case Nil
+  then show ?case 
+    by simp
+next
+  case (Cons w ws)
+  then consider "w \<notin> U" | "\<not> set ws \<subseteq> U"
+    by auto
+  then show ?case
+  proof (cases)
+    case 1
+    then have "steps (nfa_univ_trans q U) [w] q = {}"
+      by (auto simp: nfa_univ_trans_def Steps_def Step_def step_def)
+    moreover have "Steps (nfa_univ_trans q U) ws {} = {}"
+      by (meson Steps_path ex_in_conv)
+    ultimately show ?thesis
+      by (metis Steps_split all_not_in_conv append_Cons append_Nil)
+  next
+    case 2
+    then have "steps (nfa_univ_trans q U) ws q = {}"
+      using Cons by simp
+    moreover have "steps (nfa_univ_trans q U) [w] q \<subseteq> {q}"
+      by (cases "w \<in> U") (auto simp: nfa_univ_trans_def Steps_def Step_def step_def)
+    ultimately show ?thesis
+      by (metis Steps_def Steps_subset Un_insert_right ex_in_conv fold_simps(1,2) insert_absorb insert_not_empty sup.absorb_iff1)
+  qed
+qed
+
+lemmas nfa_univ_trans_correct = nfa_univ_trans_correct1 nfa_univ_trans_correct2
+
+definition nfa_univ :: "'a set \<Rightarrow> (unit, 'a) nfa" where
+  "nfa_univ U \<equiv> \<lparr>
+    transitions = nfa_univ_trans () U,
+    start = (),
+    finals = {()}
+  \<rparr>"
+
+lemma nfa_univ_lang[simp]: "nfa_lang (nfa_univ U) = {w. set w \<subseteq> U}"
+proof -
+  define \<delta> where "\<delta> \<equiv> nfa_univ_trans () U"
+  have "\<And>w. set w \<subseteq> U \<longleftrightarrow> () \<in> steps \<delta> w ()"
+    unfolding \<delta>_def using nfa_univ_trans_correct by fast
+  then show ?thesis
+    by (auto simp: \<delta>_def nfa_univ_def)
+qed
+
+subsubsection\<open>Fixed Character with arbitrary prefix/suffix\<close>
+
+text\<open>
+  Similarily to the automaton above, this automaton accepts exactly those words,
+  that contain a specific letter \<open>c\<close> at some point, and whose prefix and suffix
+  are contained within the provided alphabets \<open>PU\<close> and \<open>SU\<close>.
+\<close>
+
+definition nfa_fixc_ps_trans :: "'a \<Rightarrow> 'a set \<Rightarrow> 'a set \<Rightarrow> (nat \<times> 'a \<times> nat) set" where
+  "nfa_fixc_ps_trans c PU SU \<equiv> nfa_univ_trans 0 PU \<union> {(0, c, 1)} \<union> nfa_univ_trans 1 SU"
+
+lemma nfa_fixc_ps_trans_fin: "finite PU \<Longrightarrow> finite SU \<Longrightarrow> finite (nfa_fixc_ps_trans c PU SU)"
+  by (auto intro: nfa_univ_trans_fin simp: nfa_fixc_ps_trans_def)
+
+lemma nfa_fixc_ps_trans_correct1:
+  "(\<exists>p s. w = p@[c]@s \<and> set p \<subseteq> PU \<and> set s \<subseteq> SU) \<Longrightarrow> 1 \<in> steps (nfa_fixc_ps_trans c PU SU) w 0"
+proof -
+  assume "\<exists>p s. w = p@[c]@s \<and> set p \<subseteq> PU \<and> set s \<subseteq> SU"
+  then obtain p s where "w = p@[c]@s" and "set p \<subseteq> PU" and "set s \<subseteq> SU"
+    by blast
+  moreover have "0 \<in> steps (nfa_fixc_ps_trans c PU SU) p 0"
+    by (metis calculation(2) nfa_fixc_ps_trans_def nfa_steps_union nfa_univ_trans_correct1 singletonI)
+  moreover have "1 \<in> steps (nfa_fixc_ps_trans c PU SU) [c] 0"
+    unfolding nfa_fixc_ps_trans_def Steps_def Step_def step_def by force
+  moreover have "1 \<in> steps (nfa_fixc_ps_trans c PU SU) s 1"
+    by (metis calculation(3) inf_sup_ord(3) insertI1 nfa_fixc_ps_trans_def nfa_steps_mono nfa_univ_trans_correct1 sup_commute)
+  ultimately show "1 \<in> steps (nfa_fixc_ps_trans c PU SU) w 0"
+    using Steps_join by meson
+qed
+
+lemma nfa_fixc_ps_trans_correct2:
+  assumes "1 \<in> steps (nfa_fixc_ps_trans c PU SU) w 0"
+  shows "\<exists>p s. w = p@[c]@s \<and> set p \<subseteq> PU \<and> set s \<subseteq> SU"
+proof -
+  define \<delta>\<^sub>A where [simp]: "\<delta>\<^sub>A \<equiv> nfa_univ_trans (0::nat) PU"
+  define \<delta>\<^sub>B where [simp]: "\<delta>\<^sub>B \<equiv> nfa_univ_trans (1::nat) SU"
+
+  have "1 \<in> steps (\<delta>\<^sub>A \<union> {(0, c, 1)} \<union> \<delta>\<^sub>B) w 0"
+    using assms by (simp add: nfa_fixc_ps_trans_def)
+  then have "\<exists>w\<^sub>A w\<^sub>B. w = w\<^sub>A@[c]@w\<^sub>B \<and> 0 \<in> steps \<delta>\<^sub>A w\<^sub>A 0 \<and> 1 \<in> steps \<delta>\<^sub>B w\<^sub>B 1"
+    by (intro nfa_merge[where A="{0}" and B="{1}"]) (simp add: nfa_univ_trans_def)+
+  then obtain w\<^sub>A w\<^sub>B where w_split: "w = w\<^sub>A@[c]@w\<^sub>B" and "0 \<in> steps \<delta>\<^sub>A w\<^sub>A 0" and "1 \<in> steps \<delta>\<^sub>B w\<^sub>B 1"
+    by blast
+  then have "set w\<^sub>A \<subseteq> PU" and "set w\<^sub>B \<subseteq> SU"
+    using nfa_univ_trans_correct2 by fastforce+
+  then show ?thesis
+    using w_split by blast
+qed
+
+lemmas nfa_fixc_ps_trans_correct = nfa_fixc_ps_trans_correct1 nfa_fixc_ps_trans_correct2
+
+definition nfa_fixc_ps :: "'a \<Rightarrow> 'a set \<Rightarrow> (nat, 'a) nfa" where
+  "nfa_fixc_ps c U \<equiv> \<lparr>
+    transitions = nfa_fixc_ps_trans c U U,
+    start = 0,
+    finals = {1}
+  \<rparr>"
+
+lemma nfa_fixc_ps_lang: "nfa_lang (nfa_fixc_ps c U) = { \<alpha>@[c]@\<beta> | \<alpha> \<beta>. set \<alpha> \<subseteq> U \<and> set \<beta> \<subseteq> U }"
+  using nfa_fixc_ps_trans_correct unfolding nfa_fixc_ps_def
+  by (metis (lifting) disjoint_insert(2) inf_bot_right select_convs(1,2,3))
+
+subsubsection\<open>Singleton Language\<close>
+
+text\<open>
+  Last but not least, the automaton accepting exactly a single word can be inductively defined.
+\<close>
+
+lemma nfa_steps_empty_trans: "w \<noteq> [] \<Longrightarrow> steps {} w q\<^sub>0 = {}"
+proof (induction w)
+  case Nil
+  then show ?case
+    by simp
+next
+  case (Cons w ws)
+  moreover have "Steps {} [w] {q\<^sub>0} = {}"
+    by (simp add: Steps_def Step_def step_def)
+  moreover have "Steps {} ws {} = {}"
+    using Steps_noState by fast
+  ultimately show ?case
+    by (simp add: Steps_def)
+qed
+
+fun nfa_word_trans :: "'a list \<Rightarrow> (nat \<times> 'a \<times> nat) set" where
+  "nfa_word_trans (w#ws) = nfa_word_trans ws \<union> {(Suc (length ws), w, length ws)}" |
+  "nfa_word_trans [] = {}"
+
+lemma nfa_word_trans_domain:
+  "(q, c, q') \<in> nfa_word_trans ws \<Longrightarrow> q \<le> length ws \<and> q' \<le> length ws"
+  by (induction ws) auto
+
+definition nfa_word :: "'a list \<Rightarrow> (nat, 'a) nfa" where
+  "nfa_word ws \<equiv> \<lparr> transitions = nfa_word_trans ws, start = length ws, finals = {0} \<rparr>"
+
+lemma nfa_word_trans_correct1:
+  "0 \<in> steps (nfa_word_trans ws) ws (length ws)"
+proof (induction ws)
+  case Nil
+  then show ?case
+    by (simp add: Steps_def)
+next
+  case (Cons w ws)
+  have "0 \<in> steps (nfa_word_trans ws) ws (length ws)"
+    using Cons.IH(1) by blast
+  then have "0 \<in> steps (nfa_word_trans (w#ws)) ws (length ws)"
+    using nfa_steps_mono by (metis nfa_word_trans.simps(1) sup_ge1)
+  moreover have "length ws \<in> steps (nfa_word_trans (w#ws)) [w] (Suc (length ws))"
+  proof -
+    have "(Suc (length ws), w, length ws) \<in> nfa_word_trans (w#ws)"
+      by simp
+    then show ?thesis
+      unfolding Steps_def Step_def step_def by force
+  qed
+  ultimately show ?case
+    using Steps_join by force
+qed
+
+lemma nfa_word_trans_correct2:
+  "0 \<in> steps (nfa_word_trans ws) ws' (length ws) \<Longrightarrow> ws = ws'"
+proof (induction ws arbitrary: ws')
+  case Nil
+  then show ?case
+    by (simp, metis equals0D nfa_steps_empty_trans)
+next
+  case (Cons w ws)
+
+  \<comment> \<open>Preparation to use \texttt{nfa\_merge} lemma:\<close>
+  define \<delta>\<^sub>B where [simp]: "\<delta>\<^sub>B \<equiv> nfa_word_trans ws"
+  define B where [simp]: "B \<equiv> {n. n \<le> length ws}"
+  define \<delta> where [simp]: "\<delta> \<equiv> {} \<union> {(Suc (length ws), w, length ws)} \<union> \<delta>\<^sub>B"
+
+  \<comment> \<open>Apply the \texttt{nfa\_merge} lemma:\<close>
+  have "0 \<in> steps \<delta> ws' (length (w#ws))"
+    using Cons.prems by simp
+  moreover have "\<forall>(q, c, q')\<in>\<delta>\<^sub>B. q \<in> B \<and> q' \<in> B"
+    using nfa_word_trans_domain by force
+  ultimately have "\<exists>w\<^sub>A w\<^sub>B. ws' = w\<^sub>A@[w]@w\<^sub>B \<and> (Suc (length ws)) \<in> steps {} w\<^sub>A (Suc (length ws)) \<and> 0 \<in> steps \<delta>\<^sub>B w\<^sub>B (length ws)"
+    by (intro nfa_merge[where A="{Suc (length ws)}" and B=B]) simp+
+  then obtain w\<^sub>A w\<^sub>B where ws'_split: "ws' = w\<^sub>A@[w]@w\<^sub>B"
+      and w\<^sub>A_step: "(length (w#ws)) \<in> steps {} w\<^sub>A (length (w#ws))"
+      and w\<^sub>B_step: "0 \<in> steps \<delta>\<^sub>B w\<^sub>B (length ws)"
+    by force
+
+  \<comment> \<open>Deduce that \<open>w\<^sub>A = []\<close>:\<close>
+  have "w\<^sub>A = []"
+    using w\<^sub>A_step nfa_steps_empty_trans by fast
+
+  \<comment> \<open>Use IH to show that \<open>w\<^sub>B = ws\<close>:\<close>
+  have "ws = w\<^sub>B"
+    by (intro Cons.IH, use w\<^sub>B_step in simp)
+
+  then show ?case
+    using ws'_split by (simp add: \<open>w\<^sub>A = []\<close> \<open>ws = w\<^sub>B\<close>)
+qed
+
+lemmas nfa_word_trans_correct = nfa_word_trans_correct1 nfa_word_trans_correct2
+
+lemma nfa_word_lang[simp]: "nfa_lang (nfa_word w) = {w}"
+  unfolding nfa_word_def using nfa_word_trans_correct[of w] by fastforce
+
+lemma nfa_word_finite_trans: "finite (transitions (nfa_word w))"
+proof -
+  have "finite (nfa_word_trans w)"
+    by (induction w) simp+
+  then show ?thesis
+    by (simp add: nfa_word_def)
 qed
 
 end \<comment>\<open>end-theory FiniteAutomaton\<close>
